common/theories/Notes.md
@@ -1,0 +1,24 @@
+
+# Notes réu jeudi:
+-> sub an arg => principle
+-> pos => need the same number of var
+-> nesting => condition sp uparams v.s. sp nuparams
+
+
+# To do:
+1. finish specilisation + pos
+2. figure out isses indices
+3. wrapper function
+4. adapt regular pos + back and forth
+5. adapt metatheory with new regular pos
+
+# 2 files
+view_ind.v
+- view
+- positivty + on_inductive
+- back and forth regular def
+
+mutual_to_nested.v
+- translatation
+- preserves pos
+- preserves on ???
